Add more to the functional model of sbf.

examples/sbf/AbsFilter.v
@@ -271,27 +271,118 @@ Qed.
 
 End Frame.
 
+#[global] Instance frame_Inhabitant: Inhabitant frame := Normal [].
+
+Section sliding_mixin.
+
+  Context (frames: list frame).
+  Context (num_frames: Z).
+  Context (clear_index insert_index: Z).
+
+  Record SlidingMixin := {
+      clear_index_range: 0 <= clear_index < num_frames;
+      insert_index_range: 0 <= insert_index < num_frames;
+      insert_clear_diff: insert_index <> clear_index;
+      frame_size: Zlength frames = num_frames;
+      clear_row_status: forall l, Znth clear_index frames <> Normal l;
+      other_row_status: forall i, 0 <= i < num_frames -> i <> clear_index ->
+                             forall j, Znth i frames <> Clear j;
+  }.
+
+End sliding_mixin.
+
 Section Sliding.
 
-  #[global] Instance frame_Inhabitant: Inhabitant frame := Normal [].
+  Lemma frame_insert_None_impsbl:
+    forall (frames : list frame) (v : header_type)
+      (num_frames clear_index insert_index : Z),
+      SlidingMixin frames num_frames clear_index insert_index ->
+      frame_insert (Znth insert_index frames) v = None -> False.
+  Proof.
+    intros frames v num_frames clear_index insert_index Hs H.
+    pose proof (other_row_status _ _ _ _ Hs _
+                  (insert_index_range _ _ _ _ Hs)
+                  (insert_clear_diff _ _ _ _ Hs)).
+    unfold frame_insert, row_insert in H. destruct (Znth insert_index frames) eqn:?H.
+    - exfalso. apply (H0 i). auto.
+    - inversion H.
+  Qed.
+
+  Lemma frame_insert_Some_f_not_Clear:
+    forall (frames : list frame) (v : header_type) (num_frames clear_index insert_index : Z),
+      SlidingMixin frames num_frames clear_index insert_index ->
+      forall f : frame,
+        frame_insert (Znth insert_index frames) v = Some f -> forall j : Z, f <> Clear j.
+  Proof.
+    intros ????? Hs f H ?. destruct (Znth insert_index frames) eqn:?H.
+    - exfalso. eapply (other_row_status _ _ _ _ Hs insert_index); eauto.
+      + eapply insert_index_range; eauto.
+      + eapply insert_clear_diff; eauto.
+    - simpl in H. inversion H. intro. inversion H1.
+  Qed.
+
+  Definition window_insert'
+    (frames: list frame) (v: header_type) (num_frames clear_index insert_index: Z)
+    (Hs: SlidingMixin frames num_frames clear_index insert_index):
+    { frame | forall j, frame <> Clear j}.
+  Proof.
+    destruct (frame_insert (Znth insert_index frames) v) eqn:?H .
+    - exists f. eapply frame_insert_Some_f_not_Clear; eauto.
+    - exfalso. eapply frame_insert_None_impsbl; eauto.
+  Defined.
+
+  Lemma window_insert'_preserve:
+    forall (frames: list frame) (v: header_type) (num_frames clear_index insert_index: Z)
+      (Hs: SlidingMixin frames num_frames clear_index insert_index),
+      SlidingMixin (upd_Znth insert_index frames
+                      (proj1_sig
+                         (window_insert' frames v num_frames clear_index insert_index Hs)))
+        num_frames clear_index insert_index.
+  Proof.
+    intros. split.
+    - eapply clear_index_range; eauto.
+    - eapply insert_index_range; eauto.
+    - eapply insert_clear_diff; eauto.
+    - rewrite Zlength_upd_Znth. eapply frame_size; eauto.
+    - intros. rewrite Znth_upd_Znth_diff.
+      + eapply clear_row_status; eauto.
+      + intro. symmetry in H. revert H. eapply insert_clear_diff; eauto.
+    - intros. destruct (Z.eq_dec i insert_index).
+      + subst. rewrite Znth_upd_Znth_same; auto.
+        * remember (window_insert' frames v num_frames clear_index insert_index Hs).
+          destruct s. simpl. apply n.
+        * erewrite frame_size; eauto.
+      + rewrite Znth_upd_Znth_diff; auto. eapply other_row_status; eauto.
+  Qed.
 
   Record SlidingWindow := {
       frames: list frame;
       num_frames: Z;
       clear_index: Z;
       insert_index: Z;
-      clear_row_status: exists j, Znth clear_index frames = Clear j;
-      other_row_status: forall i, 0 <= i < num_frames -> i <> clear_index ->
-                             exists l, Znth i frames = Normal l;
-      frame_size: Zlength frames = num_frames;
-      clear_idx_range: 0 <= clear_index < num_frames;
-      insert_idx_range: 0 <= insert_index < num_frames;
-      insert_clear_diff: clear_index <> insert_index;
+      sliding_mixin: SlidingMixin frames num_frames clear_index insert_index;
     }.
 
-  Definition window_insert (win: SlidingWindow) (h: header_type): SlidingWindow.
-  Proof.
-  Abort.
+  Definition window_insert (win: SlidingWindow) (v: header_type): SlidingWindow :=
+    Build_SlidingWindow
+      (upd_Znth (insert_index win) (frames win)
+         (proj1_sig
+            (window_insert' (frames win) v
+               (num_frames win) (clear_index win) (insert_index win) (sliding_mixin win))))
+      (num_frames win) (clear_index win) (insert_index win)
+      (window_insert'_preserve (frames win) v
+         (num_frames win) (clear_index win) (insert_index win) (sliding_mixin win)).
+
+  Fixpoint remove_option {A: Type} (l: list (option A)) : list A :=
+    match l with
+    | nil => nil
+    | None :: l' => remove_option l'
+    | Some a :: l' => a :: remove_option l'
+    end.
+
+  Definition window_query (win: SlidingWindow)
+    (hashes: list (header_type -> Z)) (h: header_type) :=
+    fold_orb (remove_option (map (fun f => frame_query hashes f h) (frames win))).
 
 End Sliding.
 
